\documentclass{article}
\usepackage{epsfig}
\pagestyle{empty}
\begin{document}
$ m - b/(e^{b/m}-1) $
\pagebreak

$ \alpha e^{-\alpha x} $
\pagebreak

$ \alpha = \frac{1}{mean} $
\pagebreak

$ \alpha e^{-\alpha x} \quad x \in [0,b] $
\pagebreak

$ 1/\alpha - b/(e^{\alpha \, b}-1) $
\pagebreak

$x_m$
\pagebreak

$ k \frac{x_m^k}{x^{k+1}}$
\pagebreak

$x_m > 0$
\pagebreak

$ k > 0$
\pagebreak

$ x_m $
\pagebreak

$ k $
\pagebreak

$ x_m = mean \frac{k-1}{k}, k > 1$
\pagebreak

$ \frac{k}{\lambda}\left(\frac{x}{\lambda}\right)^{k-1}e^{-\left(\frac{x}{\lambda}\right)^k} $
\pagebreak

$ \lambda > 0$
\pagebreak

$ mean = \lambda\Gamma\left(1+\frac{1}{k}\right) $
\pagebreak

$ \Gamma $
\pagebreak

$ \frac{1}{\sigma\sqrt{2\pi}} e^{-\frac{(x-\mu)^2}{s\sigma^2}}$
\pagebreak

$ mean = \mu $
\pagebreak

$ variance = \sigma^2 $
\pagebreak

$ \frac{1}{x\sigma\sqrt{2\pi}} e^{-\frac{(ln(x) - \mu)^2}{2\sigma^2}}$
\pagebreak

$ mean = e^{\mu+\frac{\sigma^2}{2}} $
\pagebreak

$ variance = (e^{\sigma^2}-1)e^{2\mu+\sigma^2}$
\pagebreak

$ \mu $
\pagebreak

$ \sigma $
\pagebreak

$ \mu = ln(mean) - \frac{1}{2}ln\left(1+\frac{variance}{mean^2}\right)$
\pagebreak

$ \sigma = \sqrt{ln\left(1+\frac{variance}{mean^2}\right)}$
\pagebreak

$ x^{\alpha-1} \frac{e^{-\frac{x}{\beta}}}{\beta^\alpha \Gamma(\alpha)}$
\pagebreak

$ mean = \alpha\beta $
\pagebreak

$ variance = \alpha \beta^2$
\pagebreak

$ \frac{x^{k-1} e^{-\frac{x}{\lambda}}}{\lambda^k (k-1)!}$
\pagebreak

$ mean = k \lambda $
\pagebreak

$ variance = k \lambda^2$
\pagebreak

$ \alpha > 0 $
\pagebreak

$ N \in \{1,2,3 \dots\}$
\pagebreak

$ f(k; \alpha, N) = k^{-\alpha}/ H_{N,\alpha} $
\pagebreak

$ H_{N,\alpha} = \sum_{n=1}^N n^{-\alpha} $
\pagebreak

$ \alpha > 1 $
\pagebreak

$ f(k; \alpha) = k^{-\alpha}/\zeta(\alpha) $
\pagebreak

$ \zeta(\alpha) $
\pagebreak

$ \sum_{n=1}^\infty n^{-\alpha} ) $
\pagebreak

\end{document}
